Starting again (from scratch)

formalization/mfotl/thys/Proof_System.thy
@@ -1,5 +1,5 @@
 theory Proof_System
-  imports MFOTL_Monitor.Interval MFOTL_Monitor.MFOTL 
+  imports MFOTL
 begin
 
 definition ETP:: "'a trace \<Rightarrow> nat \<Rightarrow> nat"  where
@@ -11,49 +11,54 @@ definition LTP:: "'a trace \<Rightarrow> nat \<Rightarrow> nat" where
 abbreviation "LTP_p \<sigma> i I \<equiv> min i (LTP \<sigma> ((\<tau> \<sigma> i) - left I))"
 abbreviation "ETP_f \<sigma> i I \<equiv> max i (ETP \<sigma> ((\<tau> \<sigma> i) + left I))"
 
-inductive SAT and VIO :: "'a MFOTL.trace \<Rightarrow> 'a MFOTL.env \<Rightarrow> nat \<Rightarrow> 'a MFOTL.formula \<Rightarrow> bool" where
-  SPred: "(r, map (MFOTL.eval_trm v) ts) \<in> \<Gamma> \<sigma> i \<Longrightarrow> SAT \<sigma> v i (MFOTL.Pred r ts)"
-| VPred: "(r, map (MFOTL.eval_trm v) ts) \<notin> \<Gamma> \<sigma> i \<Longrightarrow> VIO \<sigma> v i (MFOTL.Pred r ts)"
-| SEq: "(MFOTL.eval_trm v t1) = (MFOTL.eval_trm v t2) \<Longrightarrow> SAT \<sigma> v i (MFOTL.Eq t1 t2)"
-| VEq: "(MFOTL.eval_trm v t1) \<noteq> (MFOTL.eval_trm v t2) \<Longrightarrow> VIO \<sigma> v i (MFOTL.Eq t1 t2)"
-| SNeg: "VIO \<sigma> v i \<phi> \<Longrightarrow> SAT \<sigma> v i (MFOTL.Neg \<phi>)"
-| VNeg: "SAT \<sigma> v i \<phi> \<Longrightarrow> VIO \<sigma> v i (MFOTL.Neg \<phi>)"
-| SDisjL: "SAT \<sigma> v i \<phi> \<Longrightarrow> SAT \<sigma> v i (MFOTL.Or \<phi> \<psi>)"
-| SDisjR: "SAT \<sigma> v i \<psi> \<Longrightarrow> SAT \<sigma> v i (MFOTL.Or \<phi> \<psi>)"
-| VDisj: "VIO \<sigma> v i \<phi> \<Longrightarrow> VIO \<sigma> v i \<psi> \<Longrightarrow> VIO \<sigma> v i (MFOTL.Or \<phi> \<psi>)"
-| SNext: "mem (\<Delta> \<sigma> (i+1)) I \<Longrightarrow> SAT \<sigma> v (i+1) \<phi> \<Longrightarrow> SAT \<sigma> v i (MFOTL.Next I \<phi>)"
-| VNext: "VIO \<sigma> v (i+1) \<phi> \<Longrightarrow> VIO \<sigma> v i (MFOTL.Next I \<phi>)"
-| VNext_le: "(\<Delta> \<sigma> (i+1)) < (left I) \<Longrightarrow> VIO \<sigma> v i (MFOTL.Next I \<phi>)"
-| VNext_ge: "enat (\<Delta> \<sigma> (i+1)) > (right I) \<Longrightarrow> VIO \<sigma> v i (MFOTL.Next I \<phi>)"
-| SPrev: "i > 0 \<Longrightarrow> mem (\<Delta> \<sigma> i) I \<Longrightarrow> SAT \<sigma> v (i-1) \<phi> \<Longrightarrow> SAT \<sigma> v i (MFOTL.Prev I \<phi>)"
-| VPrev: "i > 0 \<Longrightarrow> VIO \<sigma> v (i-1) \<phi> \<Longrightarrow> VIO \<sigma> v i (MFOTL.Prev I \<phi>)"
-| VPrev_zero: "i = 0 \<Longrightarrow> VIO \<sigma> v i (MFOTL.Prev I \<phi>)"
-| VPrev_le: "i > 0 \<Longrightarrow> (\<Delta> \<sigma> i) < (left I) \<Longrightarrow> VIO \<sigma> v i (MFOTL.Prev I \<phi>)"
-| VPrev_ge: "i > 0 \<Longrightarrow> enat (\<Delta> \<sigma> i) > (right I) \<Longrightarrow> VIO \<sigma> v i (MFOTL.Prev I \<phi>)"
+inductive SAT and VIO :: "'a Extended_MFOTL.trace \<Rightarrow> 'a Extended_MFOTL.env \<Rightarrow> nat \<Rightarrow> 'a Extended_MFOTL.formula \<Rightarrow> bool" where
+  SPred: "(r, map (Extended_MFOTL.eval_trm v) trms) \<in> \<Gamma> \<sigma> i \<Longrightarrow> SAT \<sigma> v i (Extended_MFOTL.Pred r trms)"
+| VPred: "(r, map (Extended_MFOTL.eval_trm v) trms) \<notin> \<Gamma> \<sigma> i \<Longrightarrow> VIO \<sigma> v i (Extended_MFOTL.Pred r trms)"
+| SEq: "(Extended_MFOTL.eval_trm v t1) = (Extended_MFOTL.eval_trm v t2) \<Longrightarrow> SAT \<sigma> v i (Extended_MFOTL.Eq t1 t2)"
+| VEq: "(Extended_MFOTL.eval_trm v t1) \<noteq> (Extended_MFOTL.eval_trm v t2) \<Longrightarrow> VIO \<sigma> v i (Extended_MFOTL.Eq t1 t2)"
+| SNeg: "VIO \<sigma> v i \<phi> \<Longrightarrow> SAT \<sigma> v i (Extended_MFOTL.Neg \<phi>)"
+| VNeg: "SAT \<sigma> v i \<phi> \<Longrightarrow> VIO \<sigma> v i (Extended_MFOTL.Neg \<phi>)"
+| SDisjL: "SAT \<sigma> v i \<phi> \<Longrightarrow> SAT \<sigma> v i (Extended_MFOTL.Or \<phi> \<psi>)"
+| SDisjR: "SAT \<sigma> v i \<psi> \<Longrightarrow> SAT \<sigma> v i (Extended_MFOTL.Or \<phi> \<psi>)"
+| VDisj: "VIO \<sigma> v i \<phi> \<Longrightarrow> VIO \<sigma> v i \<psi> \<Longrightarrow> VIO \<sigma> v i (Extended_MFOTL.Or \<phi> \<psi>)"
+
+| SExists: "SAT \<sigma> (x # v) i \<phi> \<Longrightarrow> SAT \<sigma> v i (Extended_MFOTL.Exists \<phi>)"
+| VExists: "VIO \<sigma> (x # v) i \<phi> \<Longrightarrow> VIO \<sigma> v i (Extended_MFOTL.Exists \<phi>)"
+
+
+| SNext: "mem (\<Delta> \<sigma> (i+1)) I \<Longrightarrow> SAT \<sigma> v (i+1) \<phi> \<Longrightarrow> SAT \<sigma> v i (Extended_MFOTL.Next I \<phi>)"
+| VNext: "VIO \<sigma> v (i+1) \<phi> \<Longrightarrow> VIO \<sigma> v i (Extended_MFOTL.Next I \<phi>)"
+| VNext_le: "(\<Delta> \<sigma> (i+1)) < (left I) \<Longrightarrow> VIO \<sigma> v i (Extended_MFOTL.Next I \<phi>)"
+| VNext_ge: "enat (\<Delta> \<sigma> (i+1)) > (right I) \<Longrightarrow> VIO \<sigma> v i (Extended_MFOTL.Next I \<phi>)"
+| SPrev: "i > 0 \<Longrightarrow> mem (\<Delta> \<sigma> i) I \<Longrightarrow> SAT \<sigma> v (i-1) \<phi> \<Longrightarrow> SAT \<sigma> v i (Extended_MFOTL.Prev I \<phi>)"
+| VPrev: "i > 0 \<Longrightarrow> VIO \<sigma> v (i-1) \<phi> \<Longrightarrow> VIO \<sigma> v i (Extended_MFOTL.Prev I \<phi>)"
+| VPrev_zero: "i = 0 \<Longrightarrow> VIO \<sigma> v i (Extended_MFOTL.Prev I \<phi>)"
+| VPrev_le: "i > 0 \<Longrightarrow> (\<Delta> \<sigma> i) < (left I) \<Longrightarrow> VIO \<sigma> v i (Extended_MFOTL.Prev I \<phi>)"
+| VPrev_ge: "i > 0 \<Longrightarrow> enat (\<Delta> \<sigma> i) > (right I) \<Longrightarrow> VIO \<sigma> v i (Extended_MFOTL.Prev I \<phi>)"
 | SSince: "j \<le> i \<Longrightarrow> mem (\<tau> \<sigma> i - \<tau> \<sigma> j) I  \<Longrightarrow> SAT \<sigma> v j \<psi> \<Longrightarrow> (\<And>k. k \<in> {j <.. i}
-            \<Longrightarrow> SAT \<sigma> v k \<phi>) \<Longrightarrow> SAT \<sigma> v i (MFOTL.Since \<phi> I \<psi>)"
-| VSince_le: "\<tau> \<sigma> i < \<tau> \<sigma> 0 + left I \<Longrightarrow> VIO \<sigma> v i (MFOTL.Since \<phi> I \<psi>)"
+            \<Longrightarrow> SAT \<sigma> v k \<phi>) \<Longrightarrow> SAT \<sigma> v i (Extended_MFOTL.Since \<phi> I \<psi>)"
+| VSince_le: "\<tau> \<sigma> i < \<tau> \<sigma> 0 + left I \<Longrightarrow> VIO \<sigma> v i (Extended_MFOTL.Since \<phi> I \<psi>)"
 | VSince: "(case right I of \<infinity> \<Rightarrow> True 
             | enat b \<Rightarrow> ETP \<sigma> ((\<tau> \<sigma> i) - b) \<le> j) \<Longrightarrow> 
             j \<le> i \<Longrightarrow> (\<tau> \<sigma> 0) + left I \<le> (\<tau> \<sigma> i) \<Longrightarrow> VIO \<sigma> v j \<phi> \<Longrightarrow>
-            (\<And>k. k \<in> {j .. (LTP_p \<sigma> i I)} \<Longrightarrow> VIO \<sigma> v k \<psi>) \<Longrightarrow> VIO \<sigma> v i (MFOTL.Since \<phi> I \<psi>)"
+            (\<And>k. k \<in> {j .. (LTP_p \<sigma> i I)} \<Longrightarrow> VIO \<sigma> v k \<psi>) \<Longrightarrow> VIO \<sigma> v i (Extended_MFOTL.Since \<phi> I \<psi>)"
 | VSince_never: "j = (case right I of \<infinity> \<Rightarrow> 0 
                       | enat b \<Rightarrow> ETP \<sigma> ((\<tau> \<sigma> i) - b)) \<Longrightarrow>
                    (\<tau> \<sigma> i) \<ge> (\<tau> \<sigma> 0) + left I \<Longrightarrow> 
-                   (\<And>k. k \<in> {j .. (LTP \<sigma> ((\<tau> \<sigma> i) - left I))} \<Longrightarrow> VIO \<sigma> v k \<psi>) \<Longrightarrow> VIO \<sigma> v i (MFOTL.Since \<phi> I \<psi>)"
+                   (\<And>k. k \<in> {j .. (LTP \<sigma> ((\<tau> \<sigma> i) - left I))} \<Longrightarrow> VIO \<sigma> v k \<psi>) \<Longrightarrow> VIO \<sigma> v i (Extended_MFOTL.Since \<phi> I \<psi>)"
 | SUntil: "j \<ge> i \<Longrightarrow> mem (\<tau> \<sigma> j - \<tau> \<sigma> i) I  \<Longrightarrow> SAT \<sigma> v j \<psi> \<Longrightarrow> (\<And>k. k \<in> {i ..< j} \<Longrightarrow> SAT \<sigma> v k \<phi>)
-             \<Longrightarrow> SAT \<sigma> v i (MFOTL.Until \<phi> I \<psi>)"
+             \<Longrightarrow> SAT \<sigma> v i (Extended_MFOTL.Until \<phi> I \<psi>)"
 | VUntil: "(case right I of \<infinity> \<Rightarrow> True 
             | enat b \<Rightarrow> j \<le> LTP \<sigma> ((\<tau> \<sigma> i) + b)) \<Longrightarrow> 
-             j \<ge> i \<Longrightarrow> VIO \<sigma> v j \<phi> \<Longrightarrow> (\<And>k. k \<in> {ETP_f \<sigma> i I .. j} \<Longrightarrow> VIO \<sigma> v k \<psi>) \<Longrightarrow> VIO \<sigma> v i (MFOTL.Until \<phi> I \<psi>)"
+             j \<ge> i \<Longrightarrow> VIO \<sigma> v j \<phi> \<Longrightarrow> (\<And>k. k \<in> {ETP_f \<sigma> i I .. j} \<Longrightarrow> VIO \<sigma> v k \<psi>) \<Longrightarrow> VIO \<sigma> v i (Extended_MFOTL.Until \<phi> I \<psi>)"
 | VUntil_never: "(\<And>k. k \<in> (case right I of \<infinity> \<Rightarrow> {ETP_f \<sigma> i I ..} 
                             | enat b \<Rightarrow> {ETP_f \<sigma> i I .. LTP \<sigma> ((\<tau> \<sigma> i) + b)}) \<Longrightarrow> VIO \<sigma> v k \<psi>) \<Longrightarrow>
-                  VIO \<sigma> v i (MFOTL.Until \<phi> I \<psi>)"
+                  VIO \<sigma> v i (Extended_MFOTL.Until \<phi> I \<psi>)"
 
-lemma soundness: "(SAT \<sigma> v i \<phi> \<longrightarrow> MFOTL.sat \<sigma> v i \<phi>) \<and> (VIO \<sigma> v i \<phi> \<longrightarrow> \<not> MFOTL.sat \<sigma> v i \<phi>)"
+lemma soundness: "(SAT \<sigma> v i \<phi> \<longrightarrow> Extended_MFOTL.sat \<sigma> v i \<phi>) \<and> (VIO \<sigma> v i \<phi> \<longrightarrow> \<not> Extended_MFOTL.sat \<sigma> v i \<phi>)"
   oops
 
-lemma completeness: "(MFOTL.sat \<sigma> v i \<phi> \<longrightarrow> SAT \<sigma> v i \<phi>) \<and> (\<not> MFOTL.sat \<sigma> v i \<phi> \<longrightarrow> VIO \<sigma> v i \<phi>)"
+lemma completeness: "(Extended_MFOTL.sat \<sigma> v i \<phi> \<longrightarrow> SAT \<sigma> v i \<phi>) \<and> (\<not> Extended_MFOTL.sat \<sigma> v i \<phi> \<longrightarrow> VIO \<sigma> v i \<phi>)"
   oops
 
 end
